hack on ibackend_cv with @pkwangjoo

compiler/backend/icompile/cv/ibackend_cvScript.sml
@@ -29,8 +29,6 @@ val asm_spec' = fn th => asm_spec th |> snd;
 val _ = cv_auto_trans locationTheory.unknown_loc_def;
 
 (* translating icompile_source_to_livesets *)
-(* val _ = to_word_0_alt_def |> asm_spec' |> arch_spec |> cv_auto_trans; *)
-(* val _ = to_livesets_0_def |> asm_spec' |> cv_trans *)
 val _ = to_livesets_0_alt_def |>
   SIMP_RULE std_ss [backendTheory.word_internal_def,
   LET_DEF |> INST_TYPE [alpha |-> ``:bool``]] |> asm_spec' |> cv_auto_trans;
@@ -51,92 +49,89 @@ val _ = mk_iconfig_def |> cv_auto_trans ;
 
 val _ = init_icompile_source_to_livesets_def |> asm_spec' |> cv_auto_trans;
 
+(* translating icompile *)
+
+val _ = icompile_word_to_stack_def |> asm_spec';
+val _ = end_icompile_word_to_stack_def |> asm_spec';
+
+val (end_icompile_cake_x64_th,end_icompile_cake_x64_def) = end_icompile_cake_def |> asm_spec ;
+val _ = end_icompile_cake_x64_def |> cv_auto_trans;
+
+val _ = icompile_cake_def |> asm_spec' |> cv_auto_trans;
+
+val _ = icompile_word_to_stack_def |> asm_spec' |> cv_auto_trans;
+
+Definition ic_w2s_mk_config_def:
+  ic_w2s_mk_config k =
+    (empty_word_iconf :'a word_iconfig) with
+    <| k := k;
+      bm := (List [4w:'a word], 1);
+      sfs_list := [];
+      fs := [0] |>
+End
+
+val _ = ic_w2s_mk_config_def |> arch_spec |> cv_auto_trans;
+
+Theorem init_icompile_word_to_stack_thm:
+  init_icompile_word_to_stack asm_conf word1_init =
+  let k = asm_conf.reg_count - (5+LENGTH asm_conf.avoid_regs) in
+  let word_iconf = ic_w2s_mk_config k in
+  let (word_iconf, stack_init) = icompile_word_to_stack asm_conf word_iconf word1_init in
+  let stack_init =
+      (raise_stub_location,raise_stub k) ::
+      (store_consts_stub_location,store_consts_stub k) :: stack_init in
+    (word_iconf, stack_init)
+Proof
+  rw[init_icompile_word_to_stack_def,ic_w2s_mk_config_def]
+QED
+
+val _ = init_icompile_word_to_stack_thm |> asm_spec' |> cv_auto_trans;
+
+val _ = init_icompile_cake_def  |> SIMP_RULE std_ss [GSYM mk_iconfig_def] |> asm_spec' |> cv_auto_trans;
+
+(* Testing the cv translation *)
+
+(* basic setup *)
+val prog = hello_prog_def |> rconc;
+val prog1 = EVAL``TAKE 15 hello_prog`` |> rconc;
+val prog2 = EVAL``DROP 15 hello_prog`` |> rconc;
+
 val c = x64_backend_config_def |> concl |> lhs;
 val x64_inc_conf = backendTheory.config_to_inc_config_def
                      |> ISPEC c |> CONV_RULE (RAND_CONV EVAL) |> rconc;
 val inc_source_conf_init_vidx = EVAL “^(x64_inc_conf).inc_source_conf with init_vidx := 10000” |> rconc;
 val x64_inc_conf = EVAL “^(x64_inc_conf) with inc_source_conf := ^(inc_source_conf_init_vidx)” |> rconc;
-val prog = hello_prog_def |> rconc;
-(*
-(* init icompile *)
-val init_res = time cv_eval “init_icompile_source_to_livesets_x64 ^(x64_inc_conf)” |> rconc;
-val (ic, reg_count_and_data_and_prog) = pairSyntax.dest_pair init_res;
-val (reg_count_and_data, prog_after_init_ic) = pairSyntax.dest_pair reg_count_and_data_and_prog;
-val (reg_count, data_after_init_ic) = pairSyntax.dest_pair reg_count_and_data;
-(* # runtime: 51.2s,    gctime: 8.8s,     systime: 22.0s. *)
 
-(*
-(* one round of icompile *)
-val icompile_res_opt = time cv_eval “icompile_source_to_livesets_x64 ^ic ^prog” |> rconc;
-val icompile_res = optionSyntax.dest_some icompile_res_opt;
-val (ic', data_and_prog) = pairSyntax.dest_pair icompile_res;
-val (data_after_ic, prog_after_ic) = pairSyntax.dest_pair data_and_prog;
-(* # runtime: 5m38s,    gctime: 26.3s,     systime: 19.3s. *)
+(* init phase *)
 
-(* end icompile *)
-val end_icompile_res = time cv_eval “end_icompile_source_to_livesets_x64 ^(ic') ^(x64_inc_conf)” |> rconc;
-val (inc_conf_after_ic, data_and_prog_end_ic) = pairSyntax.dest_pair end_icompile_res;
-val (data_after_end_ic, prog_after_end_ic) = pairSyntax.dest_pair data_and_prog_end_ic;
-(*# runtime: 3m51s,    gctime: 25.7s,     systime: 1m14s. *)
-*)
+val init_ls = time cv_eval_raw “FST (SND (init_icompile_source_to_livesets_x64 ^(x64_inc_conf)))” |> rconc;
+val init_oracs = reg_allocComputeLib.get_oracle_raw reg_alloc.Irc init_ls;
 
+val init_comp = time cv_eval “init_icompile_cake_x64 ^(x64_inc_conf) ^init_oracs”;
 
-val (dest_prog, dest_prog_type) = listSyntax.dest_list prog;
+val init_ic = #1 (pairSyntax.dest_pair (optionSyntax.dest_some (rconc init_comp)));
 
-fun div_lst_into_n [] n = []
-  | div_lst_into_n xs n =
-    let val size = length xs div n in
-    if size <= 1 then [xs]
-    else
-      let
-          val (res, rest) = List.take (xs, size) |> (fn taken => (taken, List.drop (xs, size)))
-        in
-          res :: div_lst_into_n rest (n - 1)
-        end
-    end
+(* icompile phase *)
 
-val hol_type_for_lvs_data = type_of data_after_init_ic;
-val hol_type_for_lvs_prog = type_of prog_after_init_ic;
+(* prog1 *)
+val prog1_ls = time cv_eval_raw “(9n,FST (SND (case (icompile_source_to_livesets_x64 ^init_ic ^prog1) of NONE => ARB | SOME v => v)))” |> UNDISCH |> rconc;
+val prog1_oracs = reg_allocComputeLib.get_oracle_raw reg_alloc.Irc prog1_ls;
 
-(* bench mark for dividing prog into 2 parts, unsafe opening of option *)
-fun fold_icompile ic [] = ()
-  | fold_icompile ic (p :: ps) =
-    let
-      val res_opt = cv_eval “icompile_source_to_livesets_x64 ^ic ^p” |> rconc;
-      val res = optionSyntax.dest_some res_opt;
-      val (ic', data_and_prog) = pairSyntax.dest_pair res;
-    in
-      fold_icompile ic' ps
-    end
+val prog1_comp = time cv_eval “icompile_cake_x64 ^init_ic ^prog1 ^prog1_oracs”;
+val prog1_ic = #1 (pairSyntax.dest_pair (optionSyntax.dest_some (rconc prog1_comp)));
 
+(* prog2: TODO *)
 
-val prog2parts = div_lst_into_n dest_prog 2 |> map (fn ts => listSyntax.mk_list (ts, dest_prog_type))
-fun run2parts () = fold_icompile ic prog2parts;
-time run2parts ();
-(* # runtime: 6m12s,    gctime: 31.2s,     systime: 7.2s. *)
+(* end phase *)
+val end_ls = time cv_eval_raw “(9n,FST (SND (end_icompile_source_to_livesets_x64 ^prog1_ic ^(x64_inc_conf))))” |> rconc;
+val end_oracs = reg_allocComputeLib.get_oracle_raw reg_alloc.Irc end_ls;
 
-val prog3parts = div_lst_into_n dest_prog 3 |> map (fn ts => listSyntax.mk_list (ts, dest_prog_type));
-fun run3parts () = fold_icompile ic prog3parts;
-time run3parts ();
-(* # runtime: 6m26s,    gctime: 30.0s,     systime: 9.7s. *)
+val end_comp = time cv_eval “end_icompile_cake_x64 ^init_ic ^(x64_inc_conf) ^end_oracs”;
 
+(* setting up the proof *)
 
-*)
-(*
-val x = (fetch "-" "to_livesets_alt_x64_def") |> GEN_ALL
-    |> SPEC (hello_prog_def |> concl |> lhs)
-    |> SPEC (x64_inc_conf) |> concl |> lhs;
-reg_allocComputeLib.get_oracle_raw reg_alloc.Irc (cv_eval_raw x |> rconc)
-*)
-
-(*
-val init_data_raw = time cv_eval_raw “FST (SND (init_icompile_source_to_livesets_x64 ^(x64_inc_conf)))” |> rconc;
-
-val oracles = reg_allocComputeLib.get_oracle_raw reg_alloc.Irc init_data_raw;
-
-val c_oracle_tm = backendTheory.inc_set_oracle_def
-                    |> SPEC (x64_inc_conf) |> SPEC oracles;
-*)
-
+(* MATCH_MP
+  (init_icompile_icompile_end_icompile_cake |> REWRITE_RULE [GSYM AND_IMP_INTRO])
+  TODO: put theorem here *)
 
 val _ = export_theory();
